.lake/build/ir/Go/Group.c
@@ -1,0 +1,472 @@
+// Lean compiler output
+// Module: Go.Group
+// Imports: public import Init public import Go.Board
+#include <lean/lean.h>
+#if defined(__clang__)
+#pragma clang diagnostic ignored "-Wunused-parameter"
+#pragma clang diagnostic ignored "-Wunused-label"
+#elif defined(__GNUC__) && !defined(__CLANG__)
+#pragma GCC diagnostic ignored "-Wunused-parameter"
+#pragma GCC diagnostic ignored "-Wunused-label"
+#pragma GCC diagnostic ignored "-Wunused-but-set-variable"
+#endif
+#ifdef __cplusplus
+extern "C" {
+#endif
+LEAN_EXPORT uint8_t lp_SoftwareLogic__Go_Go_posMem(lean_object*, lean_object*);
+uint8_t lean_nat_dec_eq(lean_object*, lean_object*);
+LEAN_EXPORT lean_object* lp_SoftwareLogic__Go_Go_posMem___boxed(lean_object*, lean_object*);
+LEAN_EXPORT lean_object* lp_SoftwareLogic__Go_Go_insertPos(lean_object*, lean_object*);
+LEAN_EXPORT lean_object* lp_SoftwareLogic__Go_List_foldl___at___00Go_insertManyPos_spec__0(lean_object*, lean_object*);
+LEAN_EXPORT lean_object* lp_SoftwareLogic__Go_Go_insertManyPos(lean_object*, lean_object*);
+lean_object* l_List_reverse___redArg(lean_object*);
+lean_object* lp_SoftwareLogic__Go_Go_stoneAt_x3f(lean_object*, lean_object*);
+LEAN_EXPORT lean_object* lp_SoftwareLogic__Go_List_filterTR_loop___at___00Go_sameStoneNeighbors_spec__0(lean_object*, uint8_t, lean_object*, lean_object*);
+uint8_t lp_SoftwareLogic__Go_Go_instBEqStone_beq(uint8_t, uint8_t);
+LEAN_EXPORT lean_object* lp_SoftwareLogic__Go_List_filterTR_loop___at___00Go_sameStoneNeighbors_spec__0___boxed(lean_object*, lean_object*, lean_object*, lean_object*);
+lean_object* lp_SoftwareLogic__Go_Go_neighbors(lean_object*, lean_object*);
+LEAN_EXPORT lean_object* lp_SoftwareLogic__Go_Go_sameStoneNeighbors(lean_object*, uint8_t, lean_object*);
+LEAN_EXPORT lean_object* lp_SoftwareLogic__Go_Go_sameStoneNeighbors___boxed(lean_object*, lean_object*, lean_object*);
+lean_object* lean_nat_sub(lean_object*, lean_object*);
+LEAN_EXPORT lean_object* lp_SoftwareLogic__Go_Go_groupFromAux(lean_object*, uint8_t, lean_object*, lean_object*, lean_object*);
+LEAN_EXPORT lean_object* lp_SoftwareLogic__Go_Go_groupFromAux___boxed(lean_object*, lean_object*, lean_object*, lean_object*, lean_object*);
+lean_object* lean_nat_mul(lean_object*, lean_object*);
+lean_object* lean_nat_add(lean_object*, lean_object*);
+LEAN_EXPORT lean_object* lp_SoftwareLogic__Go_Go_groupFrom_x3f(lean_object*, lean_object*);
+LEAN_EXPORT lean_object* lp_SoftwareLogic__Go_Go_groupFrom_x3f___boxed(lean_object*, lean_object*);
+LEAN_EXPORT uint8_t lp_SoftwareLogic__Go_Go_posMem(lean_object* x_1, lean_object* x_2) {
+_start:
+{
+if (lean_obj_tag(x_2) == 0)
+{
+uint8_t x_3; 
+x_3 = 0;
+return x_3;
+}
+else
+{
+lean_object* x_4; lean_object* x_5; uint8_t x_6; lean_object* x_9; lean_object* x_10; lean_object* x_11; lean_object* x_12; uint8_t x_13; 
+x_4 = lean_ctor_get(x_2, 0);
+x_5 = lean_ctor_get(x_2, 1);
+x_9 = lean_ctor_get(x_1, 0);
+x_10 = lean_ctor_get(x_1, 1);
+x_11 = lean_ctor_get(x_4, 0);
+x_12 = lean_ctor_get(x_4, 1);
+x_13 = lean_nat_dec_eq(x_9, x_11);
+if (x_13 == 0)
+{
+x_6 = x_13;
+goto block_8;
+}
+else
+{
+uint8_t x_14; 
+x_14 = lean_nat_dec_eq(x_10, x_12);
+x_6 = x_14;
+goto block_8;
+}
+block_8:
+{
+if (x_6 == 0)
+{
+x_2 = x_5;
+goto _start;
+}
+else
+{
+return x_6;
+}
+}
+}
+}
+}
+LEAN_EXPORT lean_object* lp_SoftwareLogic__Go_Go_posMem___boxed(lean_object* x_1, lean_object* x_2) {
+_start:
+{
+uint8_t x_3; lean_object* x_4; 
+x_3 = lp_SoftwareLogic__Go_Go_posMem(x_1, x_2);
+lean_dec(x_2);
+lean_dec_ref(x_1);
+x_4 = lean_box(x_3);
+return x_4;
+}
+}
+LEAN_EXPORT lean_object* lp_SoftwareLogic__Go_Go_insertPos(lean_object* x_1, lean_object* x_2) {
+_start:
+{
+uint8_t x_3; 
+x_3 = lp_SoftwareLogic__Go_Go_posMem(x_1, x_2);
+if (x_3 == 0)
+{
+lean_object* x_4; 
+x_4 = lean_alloc_ctor(1, 2, 0);
+lean_ctor_set(x_4, 0, x_1);
+lean_ctor_set(x_4, 1, x_2);
+return x_4;
+}
+else
+{
+lean_dec_ref(x_1);
+return x_2;
+}
+}
+}
+LEAN_EXPORT lean_object* lp_SoftwareLogic__Go_List_foldl___at___00Go_insertManyPos_spec__0(lean_object* x_1, lean_object* x_2) {
+_start:
+{
+if (lean_obj_tag(x_2) == 0)
+{
+return x_1;
+}
+else
+{
+lean_object* x_3; lean_object* x_4; lean_object* x_5; 
+x_3 = lean_ctor_get(x_2, 0);
+lean_inc(x_3);
+x_4 = lean_ctor_get(x_2, 1);
+lean_inc(x_4);
+lean_dec_ref(x_2);
+x_5 = lp_SoftwareLogic__Go_Go_insertPos(x_3, x_1);
+x_1 = x_5;
+x_2 = x_4;
+goto _start;
+}
+}
+}
+LEAN_EXPORT lean_object* lp_SoftwareLogic__Go_Go_insertManyPos(lean_object* x_1, lean_object* x_2) {
+_start:
+{
+lean_object* x_3; 
+x_3 = lp_SoftwareLogic__Go_List_foldl___at___00Go_insertManyPos_spec__0(x_2, x_1);
+return x_3;
+}
+}
+LEAN_EXPORT lean_object* lp_SoftwareLogic__Go_List_filterTR_loop___at___00Go_sameStoneNeighbors_spec__0(lean_object* x_1, uint8_t x_2, lean_object* x_3, lean_object* x_4) {
+_start:
+{
+if (lean_obj_tag(x_3) == 0)
+{
+lean_object* x_5; 
+x_5 = l_List_reverse___redArg(x_4);
+return x_5;
+}
+else
+{
+uint8_t x_6; 
+x_6 = !lean_is_exclusive(x_3);
+if (x_6 == 0)
+{
+lean_object* x_7; lean_object* x_8; lean_object* x_9; lean_object* x_10; 
+x_7 = lean_ctor_get(x_3, 0);
+x_8 = lean_ctor_get(x_3, 1);
+x_9 = lean_ctor_get(x_1, 1);
+lean_inc(x_7);
+x_10 = lp_SoftwareLogic__Go_Go_stoneAt_x3f(x_9, x_7);
+if (lean_obj_tag(x_10) == 0)
+{
+lean_free_object(x_3);
+lean_dec(x_7);
+x_3 = x_8;
+goto _start;
+}
+else
+{
+lean_object* x_12; uint8_t x_13; uint8_t x_14; 
+x_12 = lean_ctor_get(x_10, 0);
+lean_inc(x_12);
+lean_dec_ref(x_10);
+x_13 = lean_unbox(x_12);
+lean_dec(x_12);
+x_14 = lp_SoftwareLogic__Go_Go_instBEqStone_beq(x_13, x_2);
+if (x_14 == 0)
+{
+lean_free_object(x_3);
+lean_dec(x_7);
+x_3 = x_8;
+goto _start;
+}
+else
+{
+lean_ctor_set(x_3, 1, x_4);
+{
+lean_object* _tmp_2 = x_8;
+lean_object* _tmp_3 = x_3;
+x_3 = _tmp_2;
+x_4 = _tmp_3;
+}
+goto _start;
+}
+}
+}
+else
+{
+lean_object* x_17; lean_object* x_18; lean_object* x_19; lean_object* x_20; 
+x_17 = lean_ctor_get(x_3, 0);
+x_18 = lean_ctor_get(x_3, 1);
+lean_inc(x_18);
+lean_inc(x_17);
+lean_dec(x_3);
+x_19 = lean_ctor_get(x_1, 1);
+lean_inc(x_17);
+x_20 = lp_SoftwareLogic__Go_Go_stoneAt_x3f(x_19, x_17);
+if (lean_obj_tag(x_20) == 0)
+{
+lean_dec(x_17);
+x_3 = x_18;
+goto _start;
+}
+else
+{
+lean_object* x_22; uint8_t x_23; uint8_t x_24; 
+x_22 = lean_ctor_get(x_20, 0);
+lean_inc(x_22);
+lean_dec_ref(x_20);
+x_23 = lean_unbox(x_22);
+lean_dec(x_22);
+x_24 = lp_SoftwareLogic__Go_Go_instBEqStone_beq(x_23, x_2);
+if (x_24 == 0)
+{
+lean_dec(x_17);
+x_3 = x_18;
+goto _start;
+}
+else
+{
+lean_object* x_26; 
+x_26 = lean_alloc_ctor(1, 2, 0);
+lean_ctor_set(x_26, 0, x_17);
+lean_ctor_set(x_26, 1, x_4);
+x_3 = x_18;
+x_4 = x_26;
+goto _start;
+}
+}
+}
+}
+}
+}
+LEAN_EXPORT lean_object* lp_SoftwareLogic__Go_List_filterTR_loop___at___00Go_sameStoneNeighbors_spec__0___boxed(lean_object* x_1, lean_object* x_2, lean_object* x_3, lean_object* x_4) {
+_start:
+{
+uint8_t x_5; lean_object* x_6; 
+x_5 = lean_unbox(x_2);
+x_6 = lp_SoftwareLogic__Go_List_filterTR_loop___at___00Go_sameStoneNeighbors_spec__0(x_1, x_5, x_3, x_4);
+lean_dec_ref(x_1);
+return x_6;
+}
+}
+LEAN_EXPORT lean_object* lp_SoftwareLogic__Go_Go_sameStoneNeighbors(lean_object* x_1, uint8_t x_2, lean_object* x_3) {
+_start:
+{
+lean_object* x_4; lean_object* x_5; lean_object* x_6; lean_object* x_7; 
+x_4 = lean_ctor_get(x_1, 0);
+x_5 = lp_SoftwareLogic__Go_Go_neighbors(x_4, x_3);
+x_6 = lean_box(0);
+x_7 = lp_SoftwareLogic__Go_List_filterTR_loop___at___00Go_sameStoneNeighbors_spec__0(x_1, x_2, x_5, x_6);
+return x_7;
+}
+}
+LEAN_EXPORT lean_object* lp_SoftwareLogic__Go_Go_sameStoneNeighbors___boxed(lean_object* x_1, lean_object* x_2, lean_object* x_3) {
+_start:
+{
+uint8_t x_4; lean_object* x_5; 
+x_4 = lean_unbox(x_2);
+x_5 = lp_SoftwareLogic__Go_Go_sameStoneNeighbors(x_1, x_4, x_3);
+lean_dec_ref(x_1);
+return x_5;
+}
+}
+LEAN_EXPORT lean_object* lp_SoftwareLogic__Go_Go_groupFromAux(lean_object* x_1, uint8_t x_2, lean_object* x_3, lean_object* x_4, lean_object* x_5) {
+_start:
+{
+lean_object* x_6; uint8_t x_7; 
+x_6 = lean_unsigned_to_nat(0u);
+x_7 = lean_nat_dec_eq(x_3, x_6);
+if (x_7 == 1)
+{
+lean_dec(x_4);
+lean_dec(x_3);
+return x_5;
+}
+else
+{
+if (lean_obj_tag(x_4) == 0)
+{
+lean_dec(x_3);
+return x_5;
+}
+else
+{
+uint8_t x_8; 
+x_8 = !lean_is_exclusive(x_4);
+if (x_8 == 0)
+{
+lean_object* x_9; lean_object* x_10; lean_object* x_11; lean_object* x_12; uint8_t x_13; 
+x_9 = lean_ctor_get(x_4, 0);
+x_10 = lean_ctor_get(x_4, 1);
+x_11 = lean_unsigned_to_nat(1u);
+x_12 = lean_nat_sub(x_3, x_11);
+lean_dec(x_3);
+x_13 = lp_SoftwareLogic__Go_Go_posMem(x_9, x_5);
+if (x_13 == 0)
+{
+lean_object* x_14; lean_object* x_15; 
+lean_inc(x_9);
+x_14 = lp_SoftwareLogic__Go_Go_sameStoneNeighbors(x_1, x_2, x_9);
+x_15 = lp_SoftwareLogic__Go_List_foldl___at___00Go_insertManyPos_spec__0(x_10, x_14);
+lean_ctor_set(x_4, 1, x_5);
+{
+lean_object* _tmp_2 = x_12;
+lean_object* _tmp_3 = x_15;
+lean_object* _tmp_4 = x_4;
+x_3 = _tmp_2;
+x_4 = _tmp_3;
+x_5 = _tmp_4;
+}
+goto _start;
+}
+else
+{
+lean_free_object(x_4);
+lean_dec(x_9);
+x_3 = x_12;
+x_4 = x_10;
+goto _start;
+}
+}
+else
+{
+lean_object* x_18; lean_object* x_19; lean_object* x_20; lean_object* x_21; uint8_t x_22; 
+x_18 = lean_ctor_get(x_4, 0);
+x_19 = lean_ctor_get(x_4, 1);
+lean_inc(x_19);
+lean_inc(x_18);
+lean_dec(x_4);
+x_20 = lean_unsigned_to_nat(1u);
+x_21 = lean_nat_sub(x_3, x_20);
+lean_dec(x_3);
+x_22 = lp_SoftwareLogic__Go_Go_posMem(x_18, x_5);
+if (x_22 == 0)
+{
+lean_object* x_23; lean_object* x_24; lean_object* x_25; 
+lean_inc(x_18);
+x_23 = lp_SoftwareLogic__Go_Go_sameStoneNeighbors(x_1, x_2, x_18);
+x_24 = lp_SoftwareLogic__Go_List_foldl___at___00Go_insertManyPos_spec__0(x_19, x_23);
+x_25 = lean_alloc_ctor(1, 2, 0);
+lean_ctor_set(x_25, 0, x_18);
+lean_ctor_set(x_25, 1, x_5);
+x_3 = x_21;
+x_4 = x_24;
+x_5 = x_25;
+goto _start;
+}
+else
+{
+lean_dec(x_18);
+x_3 = x_21;
+x_4 = x_19;
+goto _start;
+}
+}
+}
+}
+}
+}
+LEAN_EXPORT lean_object* lp_SoftwareLogic__Go_Go_groupFromAux___boxed(lean_object* x_1, lean_object* x_2, lean_object* x_3, lean_object* x_4, lean_object* x_5) {
+_start:
+{
+uint8_t x_6; lean_object* x_7; 
+x_6 = lean_unbox(x_2);
+x_7 = lp_SoftwareLogic__Go_Go_groupFromAux(x_1, x_6, x_3, x_4, x_5);
+lean_dec_ref(x_1);
+return x_7;
+}
+}
+LEAN_EXPORT lean_object* lp_SoftwareLogic__Go_Go_groupFrom_x3f(lean_object* x_1, lean_object* x_2) {
+_start:
+{
+lean_object* x_3; lean_object* x_4; lean_object* x_5; 
+x_3 = lean_ctor_get(x_1, 0);
+x_4 = lean_ctor_get(x_1, 1);
+lean_inc_ref(x_2);
+x_5 = lp_SoftwareLogic__Go_Go_stoneAt_x3f(x_4, x_2);
+if (lean_obj_tag(x_5) == 0)
+{
+lean_object* x_6; 
+lean_dec_ref(x_2);
+x_6 = lean_box(0);
+return x_6;
+}
+else
+{
+uint8_t x_7; 
+x_7 = !lean_is_exclusive(x_5);
+if (x_7 == 0)
+{
+lean_object* x_8; lean_object* x_9; lean_object* x_10; lean_object* x_11; lean_object* x_12; lean_object* x_13; uint8_t x_14; lean_object* x_15; 
+x_8 = lean_ctor_get(x_5, 0);
+x_9 = lean_nat_mul(x_3, x_3);
+x_10 = lean_unsigned_to_nat(1u);
+x_11 = lean_nat_add(x_9, x_10);
+lean_dec(x_9);
+x_12 = lean_box(0);
+x_13 = lean_alloc_ctor(1, 2, 0);
+lean_ctor_set(x_13, 0, x_2);
+lean_ctor_set(x_13, 1, x_12);
+x_14 = lean_unbox(x_8);
+lean_dec(x_8);
+x_15 = lp_SoftwareLogic__Go_Go_groupFromAux(x_1, x_14, x_11, x_13, x_12);
+lean_ctor_set(x_5, 0, x_15);
+return x_5;
+}
+else
+{
+lean_object* x_16; lean_object* x_17; lean_object* x_18; lean_object* x_19; lean_object* x_20; lean_object* x_21; uint8_t x_22; lean_object* x_23; lean_object* x_24; 
+x_16 = lean_ctor_get(x_5, 0);
+lean_inc(x_16);
+lean_dec(x_5);
+x_17 = lean_nat_mul(x_3, x_3);
+x_18 = lean_unsigned_to_nat(1u);
+x_19 = lean_nat_add(x_17, x_18);
+lean_dec(x_17);
+x_20 = lean_box(0);
+x_21 = lean_alloc_ctor(1, 2, 0);
+lean_ctor_set(x_21, 0, x_2);
+lean_ctor_set(x_21, 1, x_20);
+x_22 = lean_unbox(x_16);
+lean_dec(x_16);
+x_23 = lp_SoftwareLogic__Go_Go_groupFromAux(x_1, x_22, x_19, x_21, x_20);
+x_24 = lean_alloc_ctor(1, 1, 0);
+lean_ctor_set(x_24, 0, x_23);
+return x_24;
+}
+}
+}
+}
+LEAN_EXPORT lean_object* lp_SoftwareLogic__Go_Go_groupFrom_x3f___boxed(lean_object* x_1, lean_object* x_2) {
+_start:
+{
+lean_object* x_3; 
+x_3 = lp_SoftwareLogic__Go_Go_groupFrom_x3f(x_1, x_2);
+lean_dec_ref(x_1);
+return x_3;
+}
+}
+lean_object* initialize_Init(uint8_t builtin);
+lean_object* initialize_SoftwareLogic__Go_Go_Board(uint8_t builtin);
+static bool _G_initialized = false;
+LEAN_EXPORT lean_object* initialize_SoftwareLogic__Go_Go_Group(uint8_t builtin) {
+lean_object * res;
+if (_G_initialized) return lean_io_result_mk_ok(lean_box(0));
+_G_initialized = true;
+res = initialize_Init(builtin);
+if (lean_io_result_is_error(res)) return res;
+lean_dec_ref(res);
+res = initialize_SoftwareLogic__Go_Go_Board(builtin);
+if (lean_io_result_is_error(res)) return res;
+lean_dec_ref(res);
+return lean_io_result_mk_ok(lean_box(0));
+}
+#ifdef __cplusplus
+}
+#endif
