.lake/build/ir/Go/Liberty.c
@@ -1,0 +1,314 @@
+// Lean compiler output
+// Module: Go.Liberty
+// Imports: public import Init public import Go.Group
+#include <lean/lean.h>
+#if defined(__clang__)
+#pragma clang diagnostic ignored "-Wunused-parameter"
+#pragma clang diagnostic ignored "-Wunused-label"
+#elif defined(__GNUC__) && !defined(__CLANG__)
+#pragma GCC diagnostic ignored "-Wunused-parameter"
+#pragma GCC diagnostic ignored "-Wunused-label"
+#pragma GCC diagnostic ignored "-Wunused-but-set-variable"
+#endif
+#ifdef __cplusplus
+extern "C" {
+#endif
+lean_object* l_List_reverse___redArg(lean_object*);
+uint8_t lp_SoftwareLogic__Go_Go_isEmptyAt(lean_object*, lean_object*);
+LEAN_EXPORT lean_object* lp_SoftwareLogic__Go_List_filterTR_loop___at___00Go_emptyNeighbors_spec__0(lean_object*, lean_object*, lean_object*);
+LEAN_EXPORT lean_object* lp_SoftwareLogic__Go_List_filterTR_loop___at___00Go_emptyNeighbors_spec__0___boxed(lean_object*, lean_object*, lean_object*);
+lean_object* lp_SoftwareLogic__Go_Go_neighbors(lean_object*, lean_object*);
+LEAN_EXPORT lean_object* lp_SoftwareLogic__Go_Go_emptyNeighbors(lean_object*, lean_object*);
+LEAN_EXPORT lean_object* lp_SoftwareLogic__Go_Go_emptyNeighbors___boxed(lean_object*, lean_object*);
+lean_object* lp_SoftwareLogic__Go_List_foldl___at___00Go_insertManyPos_spec__0(lean_object*, lean_object*);
+LEAN_EXPORT lean_object* lp_SoftwareLogic__Go_List_foldl___at___00Go_libertiesOfGroup_spec__0(lean_object*, lean_object*, lean_object*);
+LEAN_EXPORT lean_object* lp_SoftwareLogic__Go_List_foldl___at___00Go_libertiesOfGroup_spec__0___boxed(lean_object*, lean_object*, lean_object*);
+LEAN_EXPORT lean_object* lp_SoftwareLogic__Go_Go_libertiesOfGroup(lean_object*, lean_object*);
+LEAN_EXPORT lean_object* lp_SoftwareLogic__Go_Go_libertiesOfGroup___boxed(lean_object*, lean_object*);
+lean_object* lp_SoftwareLogic__Go_Go_groupFrom_x3f(lean_object*, lean_object*);
+LEAN_EXPORT lean_object* lp_SoftwareLogic__Go_Go_libertiesAt_x3f(lean_object*, lean_object*);
+LEAN_EXPORT lean_object* lp_SoftwareLogic__Go_Go_libertiesAt_x3f___boxed(lean_object*, lean_object*);
+static lean_once_cell_t lp_SoftwareLogic__Go_Go_groupHasLiberties_x3f___closed__0_once = LEAN_ONCE_CELL_INITIALIZER;
+static lean_object* lp_SoftwareLogic__Go_Go_groupHasLiberties_x3f___closed__0;
+static lean_once_cell_t lp_SoftwareLogic__Go_Go_groupHasLiberties_x3f___closed__1_once = LEAN_ONCE_CELL_INITIALIZER;
+static lean_object* lp_SoftwareLogic__Go_Go_groupHasLiberties_x3f___closed__1;
+uint8_t l_List_isEmpty___redArg(lean_object*);
+LEAN_EXPORT lean_object* lp_SoftwareLogic__Go_Go_groupHasLiberties_x3f(lean_object*, lean_object*);
+LEAN_EXPORT lean_object* lp_SoftwareLogic__Go_Go_groupHasLiberties_x3f___boxed(lean_object*, lean_object*);
+LEAN_EXPORT lean_object* lp_SoftwareLogic__Go_List_filterTR_loop___at___00Go_emptyNeighbors_spec__0(lean_object* x_1, lean_object* x_2, lean_object* x_3) {
+_start:
+{
+if (lean_obj_tag(x_2) == 0)
+{
+lean_object* x_4; 
+x_4 = l_List_reverse___redArg(x_3);
+return x_4;
+}
+else
+{
+uint8_t x_5; 
+x_5 = !lean_is_exclusive(x_2);
+if (x_5 == 0)
+{
+lean_object* x_6; lean_object* x_7; lean_object* x_8; uint8_t x_9; 
+x_6 = lean_ctor_get(x_2, 0);
+x_7 = lean_ctor_get(x_2, 1);
+x_8 = lean_ctor_get(x_1, 1);
+lean_inc(x_6);
+x_9 = lp_SoftwareLogic__Go_Go_isEmptyAt(x_8, x_6);
+if (x_9 == 0)
+{
+lean_free_object(x_2);
+lean_dec(x_6);
+x_2 = x_7;
+goto _start;
+}
+else
+{
+lean_ctor_set(x_2, 1, x_3);
+{
+lean_object* _tmp_1 = x_7;
+lean_object* _tmp_2 = x_2;
+x_2 = _tmp_1;
+x_3 = _tmp_2;
+}
+goto _start;
+}
+}
+else
+{
+lean_object* x_12; lean_object* x_13; lean_object* x_14; uint8_t x_15; 
+x_12 = lean_ctor_get(x_2, 0);
+x_13 = lean_ctor_get(x_2, 1);
+lean_inc(x_13);
+lean_inc(x_12);
+lean_dec(x_2);
+x_14 = lean_ctor_get(x_1, 1);
+lean_inc(x_12);
+x_15 = lp_SoftwareLogic__Go_Go_isEmptyAt(x_14, x_12);
+if (x_15 == 0)
+{
+lean_dec(x_12);
+x_2 = x_13;
+goto _start;
+}
+else
+{
+lean_object* x_17; 
+x_17 = lean_alloc_ctor(1, 2, 0);
+lean_ctor_set(x_17, 0, x_12);
+lean_ctor_set(x_17, 1, x_3);
+x_2 = x_13;
+x_3 = x_17;
+goto _start;
+}
+}
+}
+}
+}
+LEAN_EXPORT lean_object* lp_SoftwareLogic__Go_List_filterTR_loop___at___00Go_emptyNeighbors_spec__0___boxed(lean_object* x_1, lean_object* x_2, lean_object* x_3) {
+_start:
+{
+lean_object* x_4; 
+x_4 = lp_SoftwareLogic__Go_List_filterTR_loop___at___00Go_emptyNeighbors_spec__0(x_1, x_2, x_3);
+lean_dec_ref(x_1);
+return x_4;
+}
+}
+LEAN_EXPORT lean_object* lp_SoftwareLogic__Go_Go_emptyNeighbors(lean_object* x_1, lean_object* x_2) {
+_start:
+{
+lean_object* x_3; lean_object* x_4; lean_object* x_5; lean_object* x_6; 
+x_3 = lean_ctor_get(x_1, 0);
+x_4 = lp_SoftwareLogic__Go_Go_neighbors(x_3, x_2);
+x_5 = lean_box(0);
+x_6 = lp_SoftwareLogic__Go_List_filterTR_loop___at___00Go_emptyNeighbors_spec__0(x_1, x_4, x_5);
+return x_6;
+}
+}
+LEAN_EXPORT lean_object* lp_SoftwareLogic__Go_Go_emptyNeighbors___boxed(lean_object* x_1, lean_object* x_2) {
+_start:
+{
+lean_object* x_3; 
+x_3 = lp_SoftwareLogic__Go_Go_emptyNeighbors(x_1, x_2);
+lean_dec_ref(x_1);
+return x_3;
+}
+}
+LEAN_EXPORT lean_object* lp_SoftwareLogic__Go_List_foldl___at___00Go_libertiesOfGroup_spec__0(lean_object* x_1, lean_object* x_2, lean_object* x_3) {
+_start:
+{
+if (lean_obj_tag(x_3) == 0)
+{
+return x_2;
+}
+else
+{
+lean_object* x_4; lean_object* x_5; lean_object* x_6; lean_object* x_7; 
+x_4 = lean_ctor_get(x_3, 0);
+lean_inc(x_4);
+x_5 = lean_ctor_get(x_3, 1);
+lean_inc(x_5);
+lean_dec_ref(x_3);
+x_6 = lp_SoftwareLogic__Go_Go_emptyNeighbors(x_1, x_4);
+x_7 = lp_SoftwareLogic__Go_List_foldl___at___00Go_insertManyPos_spec__0(x_2, x_6);
+x_2 = x_7;
+x_3 = x_5;
+goto _start;
+}
+}
+}
+LEAN_EXPORT lean_object* lp_SoftwareLogic__Go_List_foldl___at___00Go_libertiesOfGroup_spec__0___boxed(lean_object* x_1, lean_object* x_2, lean_object* x_3) {
+_start:
+{
+lean_object* x_4; 
+x_4 = lp_SoftwareLogic__Go_List_foldl___at___00Go_libertiesOfGroup_spec__0(x_1, x_2, x_3);
+lean_dec_ref(x_1);
+return x_4;
+}
+}
+LEAN_EXPORT lean_object* lp_SoftwareLogic__Go_Go_libertiesOfGroup(lean_object* x_1, lean_object* x_2) {
+_start:
+{
+lean_object* x_3; lean_object* x_4; 
+x_3 = lean_box(0);
+x_4 = lp_SoftwareLogic__Go_List_foldl___at___00Go_libertiesOfGroup_spec__0(x_1, x_3, x_2);
+return x_4;
+}
+}
+LEAN_EXPORT lean_object* lp_SoftwareLogic__Go_Go_libertiesOfGroup___boxed(lean_object* x_1, lean_object* x_2) {
+_start:
+{
+lean_object* x_3; 
+x_3 = lp_SoftwareLogic__Go_Go_libertiesOfGroup(x_1, x_2);
+lean_dec_ref(x_1);
+return x_3;
+}
+}
+LEAN_EXPORT lean_object* lp_SoftwareLogic__Go_Go_libertiesAt_x3f(lean_object* x_1, lean_object* x_2) {
+_start:
+{
+lean_object* x_3; 
+x_3 = lp_SoftwareLogic__Go_Go_groupFrom_x3f(x_1, x_2);
+if (lean_obj_tag(x_3) == 0)
+{
+return x_3;
+}
+else
+{
+uint8_t x_4; 
+x_4 = !lean_is_exclusive(x_3);
+if (x_4 == 0)
+{
+lean_object* x_5; lean_object* x_6; 
+x_5 = lean_ctor_get(x_3, 0);
+x_6 = lp_SoftwareLogic__Go_Go_libertiesOfGroup(x_1, x_5);
+lean_ctor_set(x_3, 0, x_6);
+return x_3;
+}
+else
+{
+lean_object* x_7; lean_object* x_8; lean_object* x_9; 
+x_7 = lean_ctor_get(x_3, 0);
+lean_inc(x_7);
+lean_dec(x_3);
+x_8 = lp_SoftwareLogic__Go_Go_libertiesOfGroup(x_1, x_7);
+x_9 = lean_alloc_ctor(1, 1, 0);
+lean_ctor_set(x_9, 0, x_8);
+return x_9;
+}
+}
+}
+}
+LEAN_EXPORT lean_object* lp_SoftwareLogic__Go_Go_libertiesAt_x3f___boxed(lean_object* x_1, lean_object* x_2) {
+_start:
+{
+lean_object* x_3; 
+x_3 = lp_SoftwareLogic__Go_Go_libertiesAt_x3f(x_1, x_2);
+lean_dec_ref(x_1);
+return x_3;
+}
+}
+static lean_object* _init_lp_SoftwareLogic__Go_Go_groupHasLiberties_x3f___closed__0(void) {
+_start:
+{
+uint8_t x_1; lean_object* x_2; lean_object* x_3; 
+x_1 = 1;
+x_2 = lean_box(x_1);
+x_3 = lean_alloc_ctor(1, 1, 0);
+lean_ctor_set(x_3, 0, x_2);
+return x_3;
+}
+}
+static lean_object* _init_lp_SoftwareLogic__Go_Go_groupHasLiberties_x3f___closed__1(void) {
+_start:
+{
+uint8_t x_1; lean_object* x_2; lean_object* x_3; 
+x_1 = 0;
+x_2 = lean_box(x_1);
+x_3 = lean_alloc_ctor(1, 1, 0);
+lean_ctor_set(x_3, 0, x_2);
+return x_3;
+}
+}
+LEAN_EXPORT lean_object* lp_SoftwareLogic__Go_Go_groupHasLiberties_x3f(lean_object* x_1, lean_object* x_2) {
+_start:
+{
+lean_object* x_3; 
+x_3 = lp_SoftwareLogic__Go_Go_libertiesAt_x3f(x_1, x_2);
+if (lean_obj_tag(x_3) == 0)
+{
+lean_object* x_4; 
+x_4 = lean_box(0);
+return x_4;
+}
+else
+{
+lean_object* x_5; uint8_t x_6; 
+x_5 = lean_ctor_get(x_3, 0);
+lean_inc(x_5);
+lean_dec_ref(x_3);
+x_6 = l_List_isEmpty___redArg(x_5);
+lean_dec(x_5);
+if (x_6 == 0)
+{
+lean_object* x_7; 
+x_7 = lean_obj_once(&lp_SoftwareLogic__Go_Go_groupHasLiberties_x3f___closed__0, &lp_SoftwareLogic__Go_Go_groupHasLiberties_x3f___closed__0_once, _init_lp_SoftwareLogic__Go_Go_groupHasLiberties_x3f___closed__0);
+return x_7;
+}
+else
+{
+lean_object* x_8; 
+x_8 = lean_obj_once(&lp_SoftwareLogic__Go_Go_groupHasLiberties_x3f___closed__1, &lp_SoftwareLogic__Go_Go_groupHasLiberties_x3f___closed__1_once, _init_lp_SoftwareLogic__Go_Go_groupHasLiberties_x3f___closed__1);
+return x_8;
+}
+}
+}
+}
+LEAN_EXPORT lean_object* lp_SoftwareLogic__Go_Go_groupHasLiberties_x3f___boxed(lean_object* x_1, lean_object* x_2) {
+_start:
+{
+lean_object* x_3; 
+x_3 = lp_SoftwareLogic__Go_Go_groupHasLiberties_x3f(x_1, x_2);
+lean_dec_ref(x_1);
+return x_3;
+}
+}
+lean_object* initialize_Init(uint8_t builtin);
+lean_object* initialize_SoftwareLogic__Go_Go_Group(uint8_t builtin);
+static bool _G_initialized = false;
+LEAN_EXPORT lean_object* initialize_SoftwareLogic__Go_Go_Liberty(uint8_t builtin) {
+lean_object * res;
+if (_G_initialized) return lean_io_result_mk_ok(lean_box(0));
+_G_initialized = true;
+res = initialize_Init(builtin);
+if (lean_io_result_is_error(res)) return res;
+lean_dec_ref(res);
+res = initialize_SoftwareLogic__Go_Go_Group(builtin);
+if (lean_io_result_is_error(res)) return res;
+lean_dec_ref(res);
+return lean_io_result_mk_ok(lean_box(0));
+}
+#ifdef __cplusplus
+}
+#endif
