.lake/build/ir/Go/Move.c
@@ -1,0 +1,161 @@
+// Lean compiler output
+// Module: Go.Move
+// Imports: public import Init public import Go.Capture
+#include <lean/lean.h>
+#if defined(__clang__)
+#pragma clang diagnostic ignored "-Wunused-parameter"
+#pragma clang diagnostic ignored "-Wunused-label"
+#elif defined(__GNUC__) && !defined(__CLANG__)
+#pragma GCC diagnostic ignored "-Wunused-parameter"
+#pragma GCC diagnostic ignored "-Wunused-label"
+#pragma GCC diagnostic ignored "-Wunused-but-set-variable"
+#endif
+#ifdef __cplusplus
+extern "C" {
+#endif
+uint8_t lp_SoftwareLogic__Go_Go_inBounds(lean_object*, lean_object*);
+uint8_t lp_SoftwareLogic__Go_Go_isEmptyAt(lean_object*, lean_object*);
+LEAN_EXPORT uint8_t lp_SoftwareLogic__Go_Go_legalPlaceBasic(lean_object*, lean_object*);
+LEAN_EXPORT lean_object* lp_SoftwareLogic__Go_Go_legalPlaceBasic___boxed(lean_object*, lean_object*);
+lean_object* lp_SoftwareLogic__Go_Go_resolvePlacement_x3f(lean_object*, lean_object*);
+lean_object* lp_SoftwareLogic__Go_Go_groupHasLiberties_x3f(lean_object*, lean_object*);
+LEAN_EXPORT uint8_t lp_SoftwareLogic__Go_Go_legalPlaceNoSuicide(lean_object*, lean_object*);
+LEAN_EXPORT lean_object* lp_SoftwareLogic__Go_Go_legalPlaceNoSuicide___boxed(lean_object*, lean_object*);
+LEAN_EXPORT uint8_t lp_SoftwareLogic__Go_Go_legalMove(lean_object*, lean_object*);
+LEAN_EXPORT lean_object* lp_SoftwareLogic__Go_Go_legalMove___boxed(lean_object*, lean_object*);
+LEAN_EXPORT uint8_t lp_SoftwareLogic__Go_Go_legalPlaceBasic(lean_object* x_1, lean_object* x_2) {
+_start:
+{
+lean_object* x_3; lean_object* x_4; uint8_t x_5; 
+x_3 = lean_ctor_get(x_1, 0);
+x_4 = lean_ctor_get(x_1, 1);
+x_5 = lp_SoftwareLogic__Go_Go_inBounds(x_3, x_2);
+if (x_5 == 0)
+{
+lean_dec_ref(x_2);
+return x_5;
+}
+else
+{
+uint8_t x_6; 
+x_6 = lp_SoftwareLogic__Go_Go_isEmptyAt(x_4, x_2);
+return x_6;
+}
+}
+}
+LEAN_EXPORT lean_object* lp_SoftwareLogic__Go_Go_legalPlaceBasic___boxed(lean_object* x_1, lean_object* x_2) {
+_start:
+{
+uint8_t x_3; lean_object* x_4; 
+x_3 = lp_SoftwareLogic__Go_Go_legalPlaceBasic(x_1, x_2);
+lean_dec_ref(x_1);
+x_4 = lean_box(x_3);
+return x_4;
+}
+}
+LEAN_EXPORT uint8_t lp_SoftwareLogic__Go_Go_legalPlaceNoSuicide(lean_object* x_1, lean_object* x_2) {
+_start:
+{
+uint8_t x_3; 
+lean_inc_ref(x_2);
+x_3 = lp_SoftwareLogic__Go_Go_legalPlaceBasic(x_1, x_2);
+if (x_3 == 0)
+{
+lean_dec_ref(x_2);
+lean_dec_ref(x_1);
+return x_3;
+}
+else
+{
+uint8_t x_4; lean_object* x_5; 
+x_4 = 0;
+lean_inc_ref(x_2);
+x_5 = lp_SoftwareLogic__Go_Go_resolvePlacement_x3f(x_1, x_2);
+if (lean_obj_tag(x_5) == 0)
+{
+lean_dec_ref(x_2);
+return x_4;
+}
+else
+{
+lean_object* x_6; lean_object* x_7; 
+x_6 = lean_ctor_get(x_5, 0);
+lean_inc(x_6);
+lean_dec_ref(x_5);
+x_7 = lp_SoftwareLogic__Go_Go_groupHasLiberties_x3f(x_6, x_2);
+lean_dec(x_6);
+if (lean_obj_tag(x_7) == 0)
+{
+return x_4;
+}
+else
+{
+lean_object* x_8; uint8_t x_9; 
+x_8 = lean_ctor_get(x_7, 0);
+lean_inc(x_8);
+lean_dec_ref(x_7);
+x_9 = lean_unbox(x_8);
+lean_dec(x_8);
+return x_9;
+}
+}
+}
+}
+}
+LEAN_EXPORT lean_object* lp_SoftwareLogic__Go_Go_legalPlaceNoSuicide___boxed(lean_object* x_1, lean_object* x_2) {
+_start:
+{
+uint8_t x_3; lean_object* x_4; 
+x_3 = lp_SoftwareLogic__Go_Go_legalPlaceNoSuicide(x_1, x_2);
+x_4 = lean_box(x_3);
+return x_4;
+}
+}
+LEAN_EXPORT uint8_t lp_SoftwareLogic__Go_Go_legalMove(lean_object* x_1, lean_object* x_2) {
+_start:
+{
+if (lean_obj_tag(x_2) == 0)
+{
+lean_object* x_3; uint8_t x_4; 
+x_3 = lean_ctor_get(x_2, 0);
+lean_inc_ref(x_3);
+lean_dec_ref(x_2);
+x_4 = lp_SoftwareLogic__Go_Go_legalPlaceNoSuicide(x_1, x_3);
+return x_4;
+}
+else
+{
+uint8_t x_5; 
+lean_dec_ref(x_1);
+x_5 = 1;
+return x_5;
+}
+}
+}
+LEAN_EXPORT lean_object* lp_SoftwareLogic__Go_Go_legalMove___boxed(lean_object* x_1, lean_object* x_2) {
+_start:
+{
+uint8_t x_3; lean_object* x_4; 
+x_3 = lp_SoftwareLogic__Go_Go_legalMove(x_1, x_2);
+x_4 = lean_box(x_3);
+return x_4;
+}
+}
+lean_object* initialize_Init(uint8_t builtin);
+lean_object* initialize_SoftwareLogic__Go_Go_Capture(uint8_t builtin);
+static bool _G_initialized = false;
+LEAN_EXPORT lean_object* initialize_SoftwareLogic__Go_Go_Move(uint8_t builtin) {
+lean_object * res;
+if (_G_initialized) return lean_io_result_mk_ok(lean_box(0));
+_G_initialized = true;
+res = initialize_Init(builtin);
+if (lean_io_result_is_error(res)) return res;
+lean_dec_ref(res);
+res = initialize_SoftwareLogic__Go_Go_Capture(builtin);
+if (lean_io_result_is_error(res)) return res;
+lean_dec_ref(res);
+return lean_io_result_mk_ok(lean_box(0));
+}
+#ifdef __cplusplus
+}
+#endif
